src/main/induction_step.lean
@@ -69,44 +69,125 @@ begin
     rw def_p, exact finset.min'_le _ _ p'_in_row, },
 end
 
-lemma laced_extension (n : ℕ) {S D : finset α} {l : C.label S}
+lemma find_join {n : ℕ} {S : finset α} 
+  (l : C.label S) (cup_free : ¬C.has_ncup (n + 4) S)
+  (no_join: ¬C.has_join (n + 3) (n + 2) S)
+  (o p : α) (c : list α) (m : ℕ)
+  (o_in_S : o ∈ S) (p_in_S : p ∈ S) (o_le_p : o ≤ p) 
+  (c_in_S : c.in S) (c_ncup : C.ncup m c) (c_head : p ∈ c.head') 
+  (le_m : n + 2 ≤ m) (ho : n + 2 ≤ C.beta S o) : false :=
+begin
+  rw le_iff_lt_or_eq at o_le_p, cases o_le_p with o_lt_p o_eq_p,
+  { rcases C.beta_cup S o_in_S with ⟨d, d_in_S, d_ncup, d_last⟩,
+    by_cases sop : l.slope o p,
+    { apply cup_free,
+      have dp_ncup := d_ncup.extend_right sop o_lt_p p_in_S d_in_S d_last,
+      have ineq : n + 4 ≤ C.beta S o + 1 + 1 := by linarith,
+      apply has_ncup_le ineq, use (d ++ [p]), 
+      split, exact dp_ncup, simp, tauto, },
+    { apply no_join,
+      rcases d_ncup.take_right_with_last (n + 3) o
+        (by dec_trivial) (by linarith) d_last
+        with ⟨d', d'_in_d, d'_ncup, d'_last⟩,
+      have oc_ncup := c_ncup.extend_left sop o_in_S o_lt_p c_in_S c_head,
+      rcases oc_ncup.take_left_with_head (n + 2) o 
+        (by dec_trivial) (by linarith) (by simp)
+        with ⟨c', c'_in_oc, c'_ncup, c'_head⟩,
+      use [o, d', c'], 
+      have d'_in_S := list.subset_in d'_in_d d_in_S,
+      have c'_in_S := list.subset_in c'_in_oc (by simp; tauto),
+      tauto, }, },
+  { subst o_eq_p, apply no_join,
+    rcases C.beta_cup S o_in_S with ⟨d, d_in_S, d_ncup, d_last⟩,
+    rcases d_ncup.take_right_with_last (n + 3) o
+      (by dec_trivial) (by linarith) d_last
+      with ⟨d', d'_in_d, d'_ncup, d'_last⟩,
+    rcases c_ncup.take_left_with_head (n + 2) o 
+      (by dec_trivial) (by linarith) c_head
+      with ⟨c', c'_in_c, c'_ncup, c'_head⟩,
+    use [o, d', c'],
+    have d'_in_S := list.subset_in d'_in_d d_in_S,
+    have c'_in_S := list.subset_in c'_in_c c_in_S,
+    tauto, },
+end
+
+lemma laced_extension {n : ℕ} {S D : finset α} (l : C.label S)
   (cup_free : ¬C.has_ncup (n + 4) S) (def_D : D = C.delta (n + 2) S)
-  (no_join: ¬C.has_join (n + 1 + 2) (n + 1 + 1) S)
+  (no_join: ¬C.has_join (n + 3) (n + 2) S)
   {p' r : α} (p'r_laced : C.has_laced (n + 2) (S \ D) p' r) : 
-  l.alpha p' = 1 ∧ ∃ p : α, C.has_laced (n + 3) S p r :=
+  l.alpha p' = 1 ∧ ∃ p : α, C.has_laced (n + 3) S p r ∧ 
+    p < p' ∧ l.alpha p = 0 ∧ C.beta S p = C.beta S p' :=
 begin
   rcases p'r_laced with ⟨a, b, cp', c, cr, cp'_cup, c_cup, cr_cup, 
     ⟨cp'_in_SD, c_in_SD, cr_in_SD⟩, eq_ab, cp'_last, c_head, c_last, cr_head⟩,
   have p'_in_SD := c_in_SD _ (list.mem_of_mem_head' c_head),
   have p'_in_S := (finset.sdiff_subset S D) p'_in_SD,
-  have c_in_S := (λ a ha, (finset.sdiff_subset S D) (c_in_SD a ha)),
+  have c_in_S := list.in_superset (finset.sdiff_subset S D) c_in_SD,
+  have cr_in_S := list.in_superset (finset.sdiff_subset S D) cr_in_SD,
   rw def_D at p'_in_SD,
   rcases (C.not_mem_delta p'_in_SD) with 
     p'_beta | ⟨p, p_in_delta, eq_p, p_lt_p'⟩,
-  { exfalso, apply no_join,
-    rcases C.beta_cup S p'_in_S with ⟨d, d_in_S, d_ncup, d_last⟩,
-    rcases d_ncup.take_right_with_last (n+3) p'
-      (by dec_trivial) (by linarith) d_last with 
-      ⟨d', d'_in_d, d'_cup, d'_last⟩,
-    use [p', d', c], tauto, },
-  { have p_in_S : p ∈ S := begin 
-      rw [delta, finset.mem_filter] at p_in_delta, exact p_in_delta.left end,
-    split,
-    { have ap_lt_ap' := (l.beta_eq_alpha_inc p_in_S p'_in_S eq_p).mp p_lt_p',
-      cases nat.lt_or_ge (l.alpha p') 2 with ap' ap', linarith,
-      exfalso, apply cup_free,
-      have has_cup := l.add_alpha p'_in_S c_in_S c_cup c_head,
-      apply has_ncup_le _ has_cup, linarith, },
-    { use p, have a1_le_bp' : a + 1 ≤ C.beta S p' := begin
-        have cp'_nnil : cp' ≠ [] := begin 
-          intro h, subst h, simp at cp'_last, exact cp'_last end,
-        rcases list.take_head cp'_nnil with ⟨o, cp'', eq_cp'⟩,
-        sorry,
-      end, sorry, }, },
+  { exfalso, apply C.find_join l cup_free no_join p' p' c; 
+      try { assumption }; try { simp }, },
+  have p_in_S : p ∈ S := begin 
+    rw [delta, finset.mem_filter] at p_in_delta, exact p_in_delta.left end,
+  have ap_lt_ap' := (l.beta_eq_alpha_inc p_in_S p'_in_S eq_p).mp p_lt_p',
+  have ap' : l.alpha p' = 1 := begin
+    cases nat.lt_or_ge (l.alpha p') 2 with ap' ap', linarith,
+    exfalso, apply cup_free,
+    have has_cup := l.add_alpha p'_in_S c_in_S c_cup c_head,
+    apply has_ncup_le _ has_cup, linarith, end,
+  have ap : l.alpha p = 0 := by linarith,
+  refine ⟨ap', ⟨p, _,p_lt_p', ap, eq_p⟩⟩,
+  { have a_le_bp : a ≤ C.beta S p := begin
+      rw eq_p,
+      -- Take the head o' of cp'
+      have cp'_nnil : cp' ≠ [] := begin 
+        intro h, subst h, simp at cp'_last, exact cp'_last end,
+      rcases list.take_head cp'_nnil with ⟨o', cp'', eq_cp'⟩,
+      have o'_le_p' : o' ≤ p' := cp'_cup.head'_le_last' o' p'
+        (by rw eq_cp'; simp) (by assumption),
+      have o'_in_SD : o' ∈ S \ D := by apply cp'_in_SD; rw eq_cp'; simp,
+      have o'_in_S : o' ∈ S := (finset.sdiff_subset S D) o'_in_SD,
+      rw def_D at o'_in_SD,
+      -- Locate o in delta having the same row as o'
+      rcases C.not_mem_delta o'_in_SD with le_beta | 
+        ⟨o, o_in_delta, eq_o, o_lt_o'⟩,
+      { exfalso, apply C.find_join l cup_free no_join o' p' c; 
+        try { assumption }; try { simp }, },
+      have o_in_S : o ∈ S := 
+        by rw [config.delta] at o_in_delta; 
+        exact finset.mem_of_mem_filter _ o_in_delta,
+      -- Show that the slope of o and o' is ff
+      by_cases soo' : l.slope o o',
+      { have inc := slope_tt_inc_beta soo' o_in_S o'_in_S o_lt_o',
+        rw eq_o at inc, simp at inc, exfalso, assumption, },
+      -- extend cp' to left with o
+      have cp'_in_S := list.in_superset (finset.sdiff_subset S D) cp'_in_SD,
+      have ocp'_cup : C.ncup (a + 1) (o :: cp') := begin
+        apply cp'_cup.extend_left soo'; try {assumption},
+        rw eq_cp', simp, end,
+      apply @nat.le_of_add_le_add_right 1, rw ←ocp'_cup.right,
+      apply C.cup_length_le_beta,
+      simp, split; assumption, exact ocp'_cup.left,
+      apply list.mem_last'_cons, assumption, end,
+
+    rw config.has_laced,
+    rcases C.beta_cup S p_in_S with ⟨cp, cp_in_S, cp_cup, cp_last⟩,
+    rcases cp_cup.take_right_with_last (a + 1) p
+      (by dec_trivial) (by linarith) cp_last
+      with ⟨dp, dp_in_cp, dp_cup, dp_last⟩,
+    have dp_in_S : dp.in S := list.subset_in dp_in_cp cp_in_S,
+    have spp' : ¬l.slope p p' := begin
+      intro spp',
+      have ineq := slope_tt_inc_beta spp' p_in_S p'_in_S p_lt_p', linarith,
+    end,
+    have pc_cup := c_cup.extend_left spp' p_in_S p_lt_p' c_in_S c_head,
+    use [a + 1, b, dp, p :: c, cr, dp_cup, pc_cup, cr_cup],
+    refine ⟨⟨_, by simp; tauto, _⟩, 
+      by linarith, _, by simp, list.mem_last'_cons c_last, _⟩; assumption, },
 end
 
-/- Lemma: if one has a tight cup, 
-  its left end is strictly less than the minimum value of the last row -/
 theorem main_induction_wlog (n : ℕ) :
   C.main_goal n → C.main_goal_wlog (n+1) :=
 begin
@@ -130,7 +211,7 @@ begin
     apply cap4_free, use c, split, assumption,
     apply list.in_superset _ c_in, exact finset.sdiff_subset S D, },
   swap, { intro h, rcases h with ⟨c, ⟨c_cup, c_in⟩⟩,
-    rcases c_cup.take_head_last with ⟨p, c', q, eq_c, -⟩,
+    rcases c_cup.cons_head_tail with ⟨p, c', eq_c, -⟩,
     have p_in_c : p ∈ c := by rw eq_c; left; exact rfl,
     have p_in_SD : p ∈ S \ D := c_in _ p_in_c,
     rw def_D at p_in_SD,
@@ -138,17 +219,9 @@ begin
     have c_in_S : c.in S := (λ a ha, (finset.sdiff_subset S D) (c_in a ha)),
     rcases (C.not_mem_delta p_in_SD) with 
       le_bp | ⟨o, o_in_delta, bo_eq_bp, o_lt_p⟩,
-    { apply no_join, 
-      rcases C.beta_cup S p_in_S with ⟨d, d_in_S, d_ncup, d_last⟩,
-      rcases d_ncup.take_right_with_last (n+3) p
-        (by dec_trivial) (by linarith) d_last with 
-        ⟨d', d'_in_d, d'_cup, d'_last⟩,
-      use [p, d', p :: c'], split,
-      refine ⟨by assumption, _, by assumption⟩,
-      intros a ha, exact d_in_S _ (d'_in_d ha),
-      refine ⟨_, _, by simp⟩,
-      convert c_cup.init using 1, rw eq_c, simp,
-      rw eq_c at c_in_S, simp at ⊢ c_in_S, tauto, },
+    { apply C.find_join l cup_free no_join p p c; 
+        try {assumption}; try {simp},
+      rw eq_c, simp, },
     { have o_in_S : o ∈ S := begin 
         rw [delta, finset.mem_filter] at o_in_delta, 
         exact o_in_delta.left end,
@@ -157,9 +230,24 @@ begin
       apply cup_free, ring_nf at ⊢ has_cup,
       apply has_ncup_le _ has_cup, linarith, }, },
   { rcases t with ⟨p', q', r, s, 
-      ⟨⟨p'_lt_q', q'_le_r, r_lt_s⟩, ⟨laced_pr, laced_qs⟩⟩⟩,
-    sorry,
-     },
+      ⟨⟨p'_lt_q', q'_le_r, r_lt_s⟩, ⟨p'r_laced, q's_laced⟩⟩⟩,
+    rcases C.laced_extension l cup_free def_D no_join p'r_laced with
+      ⟨ap', ⟨p, pr_laced, p_lt_p', ap, bp⟩⟩,
+    rcases C.laced_extension l cup_free def_D no_join q's_laced with
+      ⟨aq', ⟨q, qs_laced, q_lt_q', aq, bq⟩⟩,
+    rcases pr_laced.mem_ends with ⟨p_in_S, r_in_S⟩,
+    rcases qs_laced.mem_ends with ⟨q_in_S, s_in_S⟩,
+    have p'_in_S := (finset.sdiff_subset S D) p'r_laced.mem_ends.left,
+    have q'_in_S := (finset.sdiff_subset S D) q's_laced.mem_ends.left,
+    refine ⟨p, q, r, s, ⟨⟨_, _, r_lt_s⟩, pr_laced, qs_laced⟩⟩,
+    { have ap_eq_aq := eq.trans ap aq.symm,
+      rw C.alpha_eq_beta_inc p_in_S q_in_S ap_eq_aq,
+      rw [bp, bq],
+      have ap'_eq_aq' := eq.trans ap' aq'.symm,
+      rw ←(C.alpha_eq_beta_inc p'_in_S q'_in_S ap'_eq_aq'),
+      exact p'_lt_q', },
+    { apply le_of_lt,
+      exact lt_of_lt_of_le q_lt_q' q'_le_r, }, },
 end
 
 end config
